Intermediate/Decomposition.v
@@ -3,6 +3,7 @@ Require Import Common.Util.
 Require Import Common.Memory.
 Require Import CompCert.Events.
 Require Import CompCert.Smallstep.
+Require Import CompCert.Behaviors.
 Require Import Intermediate.Machine.
 Require Import Intermediate.GlobalEnv.
 Require Import Intermediate.CS.
@@ -11,15 +12,38 @@ Require Import Intermediate.PS.
 Import Intermediate.
 
 Section Decomposition.
-  Variable p: program.
-  Variable mainC: Component.id.
-  Variable mainP: Procedure.id.
-  Variable split: list Component.id.
+  Variables p c: program.
 
-  Let G := init_env p.
-  Let G' := init_env (PS.partialize p split).
+  Let mainC := fst (prog_main p).
+  Let mainP := snd (prog_main p).
+  Let split := map fst (NMap.elements (prog_interface p)).
+  Let G := init_genv (program_link p c (prog_main p)).
+  Let G' := init_genv (PS.partial_program p (prog_interface c)).
 
-  Inductive related_states : CS.state -> PS.state -> Prop := .
+  Inductive related_states : CS.state -> PS.state -> Prop :=
+  | ProgramControl:
+      forall gps pgps mem pmem regs pc,
+        PS.is_program_component G (Pointer.component pc) ->
+        pgps = PS.to_partial_stack gps split ->
+        PS.maps_match_on split mem pmem ->
+        related_states (gps, mem, regs, pc)
+                       (PS.PC (pgps, pmem, regs, pc))
+  | ContextControl_Normal:
+      forall gps pgps mem pmem regs pc,
+        PS.is_context_component G (Pointer.component pc) ->
+        pgps = PS.to_partial_stack gps split ->
+        PS.maps_match_on split mem pmem ->
+        related_states (gps, mem, regs, pc)
+                       (PS.CC (pgps, pmem, Pointer.component pc) PS.Normal)
+  | ContextControl_WentWrong:
+      forall gps pgps mem pmem regs pc,
+        PS.is_context_component G (Pointer.component pc) ->
+        pgps = PS.to_partial_stack gps split ->
+        PS.maps_match_on split mem pmem ->
+        (forall s' t, ~ CS.step G (gps,mem,regs,pc) t s') ->
+        ~ (forall r, CS.final_state G (gps,mem,regs,pc) r) ->
+        related_states (gps, mem, regs, pc)
+                       (PS.CC (pgps, pmem, Pointer.component pc) PS.WentWrong).
 
   Lemma initial_states_match:
     forall s1,
@@ -28,27 +52,125 @@ Section Decomposition.
       PS.initial_state G' mainC mainP s2 /\ related_states s1 s2.
   Proof.
     intros s1 Hs1_init.
-    Admitted.
+    CS.unfold_state.
+    destruct Hs1_init as [Hempty_stack [Hpc_comp [Hpc_block Hpc_offset]]].
+    destruct (NMapExtra.F.In_dec (genv_entrypoints G) mainC) as [Hprg|Hctx].
+    - exists (PS.PC (PS.to_partial_stack s split, mem, regs, pc)).
+      split.
+      + unfold PS.initial_state.
+        subst. repeat split; eauto.
+        unfold G'.
+        (* TODO prove linking doesn't create problems *)
+        admit.
+      + apply ProgramControl; auto.
+        * unfold PS.is_program_component.
+          subst mainC. rewrite Hpc_comp.
+          auto.
+        * apply PS.maps_match_on_reflexive.
+    - exists (PS.CC (PS.to_partial_stack s split, mem, Pointer.component pc)
+               PS.Normal).
+      split.
+      + unfold PS.initial_state.
+        subst. repeat split. auto.
+      + apply ContextControl_Normal; auto.
+        * unfold PS.is_context_component.
+          unfold PS.is_program_component.
+          subst mainC. rewrite Hpc_comp.
+          auto.
+        * apply PS.maps_match_on_reflexive.
+  Admitted.
 
   Lemma final_states_match:
     forall s1 s2 r,
       related_states s1 s2 ->
       CS.final_state G s1 r -> PS.final_state G' s2 r.
   Proof.
+    intros s1 s2 r Hs1s2_rel Hs1_final.
+    CS.unfold_state.
+    destruct Hs1_final as [procs [proc [Hprocs [Hproc Hinstr]]]].
+    unfold PS.final_state.
+    inversion Hs1s2_rel; subst.
+    - unfold executing. eexists. eexists. eauto.
+      repeat split; eauto.
+      + (* TODO prove linking doesn't create problems *)
+        admit.
+    - reflexivity.
+    - admit.
   Admitted.
 
-  Lemma step_simulation:
-    forall s1 s2,
-      related_states s1 s2 ->
-    forall t s1',
+  Lemma lockstep_simulation:
+    forall s1 t s1',
       CS.step G s1 t s1' ->
+    forall s2,
+      related_states s1 s2 ->
     exists s2',
       PS.step G' s2 t s2' /\ related_states s1' s2'.
   Proof.
+    intros s1 t s1' Hstep s2 Hs1s2_rel.
+    inversion Hs1s2_rel; subst;
+      inversion Hstep; subst.
+    (* the program has control and doesn't produce an event *)
+    - admit.
+    - admit.
+    - admit.
+    - admit.
+    - admit.
+    - admit.
+    - admit.
+    - admit.
+    - admit.
+    - admit.
+    - admit.
+    - admit.
+
+    (* the program has control and produces an event *)
+    - admit.
+    - admit.
+
+    (* the context has control and doesn't produce an event *)
+    - admit.
+    - admit.
+    - admit.
+    - admit.
+    - admit.
+    - admit.
+    - admit.
+    - admit.
+    - admit.
+    - admit.
+    - admit.
+    - admit.
+
+    (* the context has control and produces an event *)
+    - admit.
+    - admit.
   Admitted.
 
-  Theorem forward_sim:
-    forward_simulation (CS.sem p mainC mainP) (PS.sem (PS.partialize p split) mainC mainP).
+  Theorem PS_simulates_CS:
+    forward_simulation (CS.sem (program_link p c (prog_main p)))
+                       (PS.sem p (prog_interface c)).
+  Proof.
+    apply forward_simulation_step with related_states.
+    - apply initial_states_match.
+    - apply final_states_match.
+    - apply lockstep_simulation.
+  Qed.
+
+  Corollary PS_improves_CS_behavior:
+    forall beh1,
+      program_behaves (CS.sem (program_link p c (prog_main p))) beh1 ->
+    exists beh2,
+      program_behaves (PS.sem p (prog_interface c)) beh2 /\ behavior_improves beh1 beh2.
+  Proof.
+    intros.
+    eapply forward_simulation_behavior_improves; eauto.
+    apply PS_simulates_CS.
+  Qed.
+
+  Corollary PS_behaves_as_CS:
+    forall beh,
+      program_behaves (CS.sem (program_link p c (prog_main p))) beh ->
+      program_behaves (PS.sem p (prog_interface c)) beh.
   Proof.
   Admitted.
 End Decomposition.
