Source/Language.v
@@ -1,5 +1,7 @@
 Require Import Common.Definitions.
 Require Import Common.Values.
+Require Import Common.Memory.
+Require Import Common.Linking.
 
 Inductive expr : Type :=
 | E_val : value -> expr
@@ -17,6 +19,97 @@ Module Source.
   Record program : Type := mkProg {
     prog_interface : Program.interface;
     prog_procedures : NMap.t (NMap.t expr);
-    prog_buffers : NMap.t nat
+    prog_buffers : NMap.t nat;
+    prog_main : Component.id * Procedure.id
   }.
+
+  Definition only_allowed_calls (p: program) : bool :=
+    let fix check_expr cur_comp e :=
+        match e with
+        | E_val _ => true
+        | E_local => true
+        | E_binop _ e1 e2 =>
+          andb (check_expr cur_comp e1) (check_expr cur_comp e2)
+        | E_seq e1 e2 =>
+          andb (check_expr cur_comp e1) (check_expr cur_comp e2)
+        | E_if e1 e2 e3 =>
+          andb (andb (check_expr cur_comp e1) (check_expr cur_comp e2))
+               (check_expr cur_comp e3)
+        | E_alloc e =>
+          check_expr cur_comp e
+        | E_deref e =>
+          check_expr cur_comp e
+        | E_assign e1 e2 =>
+          andb (check_expr cur_comp e1) (check_expr cur_comp e2)
+        | E_call C' P' e =>
+          andb (orb (imported_procedure_b (prog_interface p) cur_comp C' P')
+                    (cur_comp =? C'))
+               (check_expr cur_comp e)
+        | E_exit => true
+        end
+    in
+    let fix check_procedures cur_comp procs :=
+        match procs with
+        | [] => true
+        | (_, e) :: procs' =>
+          andb (check_expr cur_comp e) (check_procedures cur_comp procs')
+        end
+    in
+    let fix check_components comps :=
+        match comps with
+        | [] => true
+        | (C, Cprocs) :: comps' =>
+          andb (check_procedures C (NMap.elements Cprocs))
+               (check_components comps')
+        end
+    in check_components (NMap.elements (prog_procedures p)).
+
+  Definition required_local_buffers (p: program) : bool :=
+    let check_for_comp C :=
+        match NMap.find C (prog_buffers p) with
+        | Some size => 0 <? size
+        | None => false
+        end
+    in
+    let fix check_components comps :=
+        match comps with
+        | [] => true
+        | (C, _) :: comps' =>
+          andb (check_for_comp C) (check_components comps')
+        end
+    in
+    check_components (NMap.elements (prog_procedures p)).
+
+  Definition valid_main (p: program) : bool :=
+    match NMap.find (fst (prog_main p)) (prog_procedures p) with
+    | Some procs => NMap.mem (snd (prog_main p)) procs
+    | None => false
+    end.
+
+  (* TODO check for interface soundness *)
+  Definition well_formed_program (p: program) : bool:=
+    (only_allowed_calls p) &&
+    (required_local_buffers p) &&
+    (valid_main p).
+
+  Fixpoint alloc_buffers
+           (bufs: list (Component.id * nat))
+           (m: Memory.t) (addrs: NMap.t Block.id)
+    : Memory.t * NMap.t Block.id :=
+    match bufs with
+    | [] => (m, addrs)
+    | (C,size)::bufs' =>
+      let memC := match NMap.find C m with
+                  | Some memC => memC
+                  | None => ComponentMemory.empty
+                  end in
+      let '(memC', b) := ComponentMemory.alloc memC size in
+      alloc_buffers bufs' (NMap.add C memC' m) (NMap.add C b addrs)
+    end.
+
+  Definition init_all (p: program) : NMap.t Block.id * Memory.t :=
+    let pbufs := NMap.elements (prog_buffers p) in
+    let init_mem := Memory.empty (map fst pbufs) in
+    let '(mem, bufs) := alloc_buffers pbufs init_mem (@NMap.empty Block.id) in
+    (bufs, mem).
 End Source.
