Source/GlobalEnv.v
@@ -2,8 +2,16 @@ Require Import Common.Definitions.
 Require Import Common.Values.
 Require Import Source.Language.
 
+Import Source.
+
 Record global_env : Type := mkGlobalEnv {
   genv_interface : Program.interface;
   genv_procedures : NMap.t (NMap.t expr);
   genv_buffers : NMap.t Block.id
 }.
+
+Definition init_genv (p: program) : global_env :=
+  let '(bufs, _) := init_all p in
+  {| genv_interface := prog_interface p;
+     genv_procedures := prog_procedures p;
+     genv_buffers := bufs |}.
